coq-inductive

coq_inductive/tll_ast.v
@@ -11,7 +11,10 @@ Delimit Scope sort_scope with srt.
 Open Scope sort_scope.
 
 Inductive sort : Type := U | L.
-Bind Scope sort_scope with sort.
+Bind Scope term_scope with sort.
+
+Inductive relv : Type := R | N.
+Bind Scope term_scope with relv.
 
 Inductive sort_leq : sort -> sort -> Prop :=
 | sort_leqU s :
@@ -21,22 +24,16 @@ Inductive sort_leq : sort -> sort -> Prop :=
 Notation "s ⊑ t" := (sort_leq s t) (at level 30) : sort_scope.
 
 Inductive term : Type :=
-| Var (x : var)
-| Sort (s : sort)
-| Pi0 (A : term) (B : {bind term}) (s : sort)
-| Pi1 (A : term) (B : {bind term}) (s : sort)
-| Lam0 (A : term) (m : {bind term}) (s : sort)
-| Lam1 (A : term) (m : {bind term}) (s : sort)
-| App0 (m n : term)
-| App1 (m n : term)
-| Ind0 (A : term) (Cs : list term) (s : sort)
-| Ind1 (A : term) (Cs : list term) (s : sort)
-| Constr0 (i : nat) (I : term) (s : sort)
-| Constr1 (i : nat) (I : term) (s : sort)
-| Case0 (m Q : term) (Fs : list term)
-| Case1 (m Q : term) (Fs : list term)
-| Fix (A : term) (m : {bind term})
-| Ptr (l : nat).
+| Var  (x : var)
+| Srt (s : sort)
+| Pi   (A : term) (B : {bind term}) (s : sort) (r : relv)
+| Lam  (A : term) (m : {bind term}) (s : sort) (r : relv)
+| App  (m n : term) (r : relv)
+| Ind  (A : term) (Cs : list term) (s : sort) (r : relv)
+| Cons (i : nat) (I : term) (s : sort) (r : relv)
+| Case (m Q : term) (Fs : list term) (r : relv)
+| Fix  (A : term) (m : {bind term})
+| Ptr  (l : nat).
 
 #[global] Instance Ids_term : Ids term. derive. Defined.
 #[global] Instance Rename_term : Rename term. derive. Defined.
@@ -46,45 +43,33 @@ Inductive term : Type :=
 Section term_ind_nested.
   Variable P : term -> Prop.
   Hypothesis ih_Var : forall x, P (Var x).
-  Hypothesis ih_Sort : forall s, P (Sort s).
-  Hypothesis ih_Pi0 : forall A B s, P A -> P B -> P (Pi0 A B s).
-  Hypothesis ih_Pi1 : forall A B s, P A -> P B -> P (Pi1 A B s).
-  Hypothesis ih_Lam0 : forall A m s, P A -> P m -> P (Lam0 A m s).
-  Hypothesis ih_Lam1 : forall A m s, P A -> P m -> P (Lam1 A m s).
-  Hypothesis ih_App0 : forall m n, P m -> P n -> P (App0 m n).
-  Hypothesis ih_App1 : forall m n, P m -> P n -> P (App1 m n).
-  Hypothesis ih_Ind0 : forall A Cs s, P A -> All1 P Cs -> P (Ind0 A Cs s).
-  Hypothesis ih_Ind1 : forall A Cs s, P A -> All1 P Cs -> P (Ind1 A Cs s).
-  Hypothesis ih_Constr0 : forall i I s, P I -> P (Constr0 i I s).
-  Hypothesis ih_Constr1 : forall i I s, P I -> P (Constr1 i I s).
-  Hypothesis ih_Case0 : forall m Q Fs, P m -> P Q -> All1 P Fs -> P (Case0 m Q Fs).
-  Hypothesis ih_Case1 : forall m Q Fs, P m -> P Q -> All1 P Fs -> P (Case1 m Q Fs).
+  Hypothesis ih_Srt : forall s, P (Srt s).
+  Hypothesis ih_Pi : forall A B s r, P A -> P B -> P (Pi A B s r).
+  Hypothesis ih_Lam : forall A m s r, P A -> P m -> P (Lam A m s r).
+  Hypothesis ih_App : forall m n r, P m -> P n -> P (App m n r).
+  Hypothesis ih_Ind : forall A Cs s r, P A -> {∀ C ∈ Cs, P C} -> P (Ind A Cs s r).
+  Hypothesis ih_Cons : forall i I s r, P I -> P (Cons i I s r).
+  Hypothesis ih_Case : forall m Q Fs r, P m -> P Q -> {∀ F ∈ Fs, P F} -> P (Case m Q Fs r).
   Hypothesis ih_Fix : forall A m, P A -> P m -> P (Fix A m).
   Hypothesis ih_Ptr : forall l, P (Ptr l).
 
   Fixpoint term_ind_nested m : P m. 
   Proof with eauto.
     have ih_nested :=
-      fix fold xs : All1 P xs :=
+      fix fold xs : {∀ x ∈ xs, P x} :=
         match xs with
-        | nil => All1_nil _
-        | x :: xs => All1_cons (term_ind_nested x) (fold xs)
+        | nil => Forall1_nil _
+        | x :: xs => Forall1_cons (term_ind_nested x) (fold xs)
         end.
     case m; move=>*.
     apply: ih_Var.
-    apply: ih_Sort.
-    apply: ih_Pi0...
-    apply: ih_Pi1...
-    apply: ih_Lam0...
-    apply: ih_Lam1...
-    apply: ih_App0...
-    apply: ih_App1...
-    apply: ih_Ind0...
-    apply: ih_Ind1...
-    apply: ih_Constr0...
-    apply: ih_Constr1...
-    apply: ih_Case0...
-    apply: ih_Case1...
+    apply: ih_Srt.
+    apply: ih_Pi...
+    apply: ih_Lam...
+    apply: ih_App...
+    apply: ih_Ind...
+    apply: ih_Cons...
+    apply: ih_Case...
     apply: ih_Fix...
     apply: ih_Ptr...
   Qed.
